.

theories/Logic/ConstructiveDomainTheory.v
@@ -9,6 +9,8 @@ Module BasicCoLaTheory.
 
   Local Existing Instances pair_isPoset arrow_isPoset.
 
+  Global Hint Constructors _image : poset_hints.
+
   Definition getInfimumOf_inCoLa {D : Type} {requiresPoset : isPoset D} {requiresCoLa : isCoLa D} (X : ensemble D) : {inf_X : D | isInfimumOf inf_X X} :=
     let inf_X : D := proj1_sig (getSupremumOf_inCoLa (LowerBoundsOf X)) in
     @exist D (fun inf : D => isInfimumOf inf X) inf_X (proj2 (SupremumOfLowerBounds_isInfimum inf_X X) (proj2_sig (getSupremumOf_inCoLa (LowerBoundsOf X))))
@@ -18,11 +20,47 @@ Module BasicCoLaTheory.
     @sig (Hask.arrow dom cod) (fun f : dom -> cod => isMonotonicMap f)
   .
 
-  Local Instance MonotonicMaps_isPoset (dom : Type) (cod : Type) {dom_requiresPoset : isPoset dom} {cod_requiresPoset : isPoset cod} : isPoset (MonotonicMaps dom cod) :=
+  Local Notation " '⟬' dom '⟶' cod '⟭' " := (MonotonicMaps dom cod) : type_scope.
+
+  Local Instance MonotonicMaps_isPoset (dom : Type) (cod : Type) {dom_requiresPoset : isPoset dom} {cod_requiresPoset : isPoset cod} : isPoset ⟬ dom ⟶ cod ⟭ :=
     subPoset (Hask.arrow dom cod) (requiresPoset := arrow_isPoset cod_requiresPoset)
   .
 
-  Local Notation " '⟬' dom '⟶' cod '⟭' " := (MonotonicMaps dom cod) : type_scope.
+  Definition supOfMonotonicMaps {dom : Type} {cod : Type} {dom_requiresPoset : isPoset dom} {cod_requiresPoset : isPoset cod} {dom_requiresCoLa : isCoLa dom} {cod_requiresCoLa : isCoLa cod} (fs : ensemble ⟬ dom ⟶ cod ⟭) : dom -> cod :=
+    fun x : dom => proj1_sig (getSupremumOf_inCoLa (image (fun f_i : ⟬ dom ⟶ cod ⟭ => proj1_sig f_i x) fs))
+  .
+
+  Lemma supOfMonotonicMaps_proj2_sig {dom : Type} {cod : Type} {dom_requiresPoset : isPoset dom} {cod_requiresPoset : isPoset cod} {dom_requiresCoLa : isCoLa dom} {cod_requiresCoLa : isCoLa cod} (fs : ensemble ⟬ dom ⟶ cod ⟭)
+    : forall x : dom, isSupremumOf (supOfMonotonicMaps fs x) (image (fun f_i : ⟬ dom ⟶ cod ⟭ => proj1_sig f_i x) fs).
+  Proof. exact (fun x : dom => proj2_sig (getSupremumOf_inCoLa (image (fun f_i : ⟬ dom ⟶ cod ⟭ => proj1_sig f_i x) fs))). Qed.
+
+  Lemma supOfMonotonicMaps_isMonotonicMap {dom : Type} {cod : Type} {dom_isPoset : isPoset dom} {cod_isPoset : isPoset cod} {dom_isCoLa : isCoLa dom} {cod_isCoLa : isCoLa cod} (fs : ensemble ⟬ dom ⟶ cod ⟭)
+    : isMonotonicMap (supOfMonotonicMaps fs).
+  Proof.
+    intros x x' x_le_x'. simpl. eapply supOfMonotonicMaps_proj2_sig with (x := x). red.
+    intros y y_in. apply in_image_iff in y_in. destruct y_in as [f [y_eq f_in]]. subst y.
+    transitivity (proj1_sig f x'); [eapply (proj2_sig f) | eapply supOfMonotonicMaps_proj2_sig with (x := x')]; eauto with *.
+  Qed.
+
+  Definition supremum_m {dom : Type} {cod : Type} {dom_isPoset : isPoset dom} {cod_isPoset : isPoset cod} {dom_isCoLa : isCoLa dom} {cod_isCoLa : isCoLa cod} (fs : ensemble ⟬ dom ⟶ cod ⟭) : ⟬ dom ⟶ cod ⟭ :=
+    @exist (dom -> cod) isMonotonicMap (supOfMonotonicMaps fs) (supOfMonotonicMaps_isMonotonicMap fs)
+  .
+
+  Lemma supremum_m_isSupremumOf {dom : Type} {cod : Type} {dom_isPoset : isPoset dom} {cod_isPoset : isPoset cod} {dom_isCoLa : isCoLa dom} {cod_isCoLa : isCoLa cod}
+    : forall fs : ensemble ⟬ dom ⟶ cod ⟭, isSupremumOf (supremum_m fs) fs.
+  Proof with eauto with *.
+    unfold supremum_m; intros fs f. split; intros ?; desnw.
+    - intros f_i f_i_in. rewrite <- SUPREMUM_LE_UPPER_BOUND.
+      intros x. simpl. eapply supOfMonotonicMaps_proj2_sig with (x := x)...
+    - intros x. simpl. eapply supOfMonotonicMaps_proj2_sig with (x := x).
+      intros y y_in. apply in_image_iff in y_in. destruct y_in as [f_i [y_eq f_i_in]]. subst y.
+      revert x. change (f_i =< f)...
+  Qed.
+
+  Local Instance MonotonicMaps_isCoLa (dom : Type) (cod : Type) {dom_isPoset : isPoset dom} {cod_isPoset : isPoset cod} {dom_isCoLa : isCoLa dom} {cod_isCoLa : isCoLa cod} : isCoLa ⟬ dom ⟶ cod ⟭ :=
+    { getSupremumOf_inCoLa (fs : ensemble ⟬ dom ⟶ cod ⟭) := @exist ⟬ dom ⟶ cod ⟭ (fun sup_fs : ⟬ dom ⟶ cod ⟭ => isSupremumOf sup_fs fs) (supremum_m fs) (supremum_m_isSupremumOf fs)
+    }
+  .
 
 End BasicCoLaTheory.
 
